Protocols/RBABC/Liveness_tla.v
@@ -26,6 +26,13 @@ Include LivenessTLA A M BTh BSett Pk PSOp RBACP Ns RBACAdv RBACN.
 Definition exec_proj1 (e : exec World) : exec RBN.Ns.World := fun n => world_proj1 (e n).
 
 Definition exec_proj2 (e : exec World) : exec ACN.Ns.World := fun n => world_proj2 (e n).
+
+Definition ssdexec_proj1 (f : exec system_step_descriptor) : exec RBN.system_step_descriptor :=
+  fun n => (ssd_proj1 (f n)).
+
+Definition exec_norm1 f (e : exec World) : exec RBN.Ns.World :=
+  RBN.final_world_n (ssdexec_proj1 f) (world_proj1 (e 0)).
+(* unique interpretability ... *)
 (*
 Definition next_proj1 (w1 w1' : RBN.Ns.World) : Prop :=
   forall q w w', system_step q w w' -> RBN.system_step (ssd_proj1 q) w1 w1'.
@@ -36,26 +43,33 @@ Proof. intros H. hnf in H |- *.
 *)
 (* TODO it seems inevitable to use some kind of choice axiom to prove the existence below?
     sounds like reasonable, since we are reasoning about infinity *)
+(*
 Fact exec_proj1_sound (e : exec World) (H : e ⊨ □ ⟨ next ⟩) :
   ∃ (e' : exec RBN.Ns.World), 
     RBLiveTLA.exec_rel e' (exec_proj1 e) ∧
     (e' ⊨ □ ⟨ RBLiveTLA.next ⟩).
-    (* (e' ⊨ □ ⟨ next_proj1 ⟩). *)
+*)
+Fact exec_proj1_sound (e : exec World) f (Hf : e ⊨ nextf f) :
+  let: e' := exec_norm1 f e in
+    RBLiveTLA.exec_rel e' (exec_proj1 e) ∧
+    (* (e' ⊨ □ ⟨ RBLiveTLA.next ⟩). *)
+    (e' ⊨ RBLiveTLA.nextf (ssdexec_proj1 f)).
 Proof.
+  (*
   autounfold with tla in H. setoid_rewrite drop_n in H. simpl in H.
   pose proof (choice _ H) as (f & Hf). clear H.   (* !!!!!!!! *)
-  pose (e' := RBN.final_world_n (fun n => (ssd_proj1 (f n))) (world_proj1 (e 0))).
-  exists e'. apply and_wlog_r.
-  - hnf. intros n. unfold exec_proj1. subst e'.
+  *)
+  autounfold with tla in Hf. hnf in Hf. apply and_wlog_r.
+  - hnf. intros n. unfold exec_proj1, exec_norm1.
     induction n as [ | n IH ]; try reflexivity.
     rewrite RBN.final_world_n_add_1.
     pose proof (ssd_proj1_sound _ _ _ (Hf n)) as (_ & H).
     rewrite -H. now apply RBN.next_world_preserves_World_rel.
   - intros Hrel.
     split_and?; autounfold with tla.
-    + intros k. exists (ssd_proj1 (f k)). rewrite !drop_n /=. 
+    + intros k. (* exists (ssd_proj1 (f k)). rewrite !drop_n /=. *)
       pose proof (ssd_proj1_sound _ _ _ (Hf k)) as (Ha & Hb).
-      subst e'. rewrite RBN.final_world_n_add_1. eapply RBN.step_mirrors_World_rel.
+      unfold exec_norm1 in *. rewrite RBN.final_world_n_add_1. eapply RBN.step_mirrors_World_rel.
       1: symmetry; apply Hrel. 1: apply Ha. 1: intros; auto. (* nice *)
       specialize (Hrel (S k)). rewrite RBN.final_world_n_add_1 in Hrel. rewrite Hb Hrel. reflexivity.
     (* + intros k. hnf. intros q w w' Hstep. rewrite !drop_n /=.
@@ -63,19 +77,30 @@ Proof.
       subst e'. rewrite RBN.final_world_n_add_1. eapply RBN.step_mirrors_World_rel. *)
 Qed.
 
-Fact exec_proj1_sound_fairness (e : exec World) (H : e ⊨ □ ⟨ next ⟩)
+(* TODO have no way to go ... this might be too strong, but I have no better idea
+    on how to avoid ambiguity. *)
+Definition disambiguation e f : Prop :=
+  forall q n, system_step q (e n) (e (S n)) → f n = q.
+
+Fact exec_proj1_sound_fairness (e : exec World) f (H : e ⊨ nextf f) (Hig : disambiguation e f)
   (e' : exec RBN.Ns.World) (Hrel : RBLiveTLA.exec_rel e' (exec_proj1 e))
-  (H' : e' ⊨ □ ⟨ RBLiveTLA.next ⟩) :
+  (* (H' : e' ⊨ □ ⟨ RBLiveTLA.next ⟩) : *)
+  (H' : e' ⊨ RBLiveTLA.nextf (ssdexec_proj1 f)) :
   (e ⊨ fairness) → (e' ⊨ RBLiveTLA.fairness).
 Proof.
-  (* change view *)
-  intros Hfair%fairness_adequate; auto. apply RBLiveTLA.fairness_adequate; auto.
+  (* change view, get k *)
+  intros Hfair%fairness_adequate; auto. 2: eapply nextf_impl_next, H. 
+  apply RBLiveTLA.fairness_adequate; auto. 1: eapply RBLiveTLA.nextf_impl_next, H'. 
   hnf in Hfair |- *. intros [ src dst msg ? ] (Hs & Hd). simpl in *. intros -> n Hin.
   specialize (Hfair (mkP src dst (inl msg) false) (conj Hs Hd) eq_refl n).
   apply (proj2 (Hrel n)) in Hin. unfold exec_proj1, world_proj1 in Hin. simpl in Hin.
   apply option_map_list_In in Hin. destruct Hin as ([ ? ? [] ? ] & Hin & Hpj); try discriminate.
   cbn in Hpj. revert Hpj. intros [= -> -> -> ->]. specialize (Hfair Hin).
   destruct Hfair as (k & Hstep). 
-Abort.
+  (* key point: the correspondence between delivery steps *)
+  exists k.
+  apply Hig in Hstep. hnf in H'. specialize (H' (k + n)). 
+  unfold ssdexec_proj1 in H'. rewrite Hstep in H'. now cbn in H'.
+Qed.
 
 End RBACLiveness2.
